@prefix : <http://crossings.github.io/term/> .
@prefix dct: <http://purl.org/dc/terms/> .
@prefix owl: <http://www.w3.org/2002/07/owl#> .
@prefix rdf: <http://www.w3.org/1999/02/22-rdf-syntax-ns#> .
@prefix xml: <http://www.w3.org/XML/1998/namespace> .
@prefix xsd: <http://www.w3.org/2001/XMLSchema#> .
@prefix rdfs: <http://www.w3.org/2000/01/rdf-schema#> .

<http://crossings.github.io/ont/martialstyle> rdf:type owl:Ontology ;
    dct:title   "The Martial Arts ontology: Stylistic framework"    ;
    dct:creator   <https://orcid.org/0000-0002-9272-908X>
.


###  http://semanticweb.org/ont/martialmotion#belongsInSystem
:belongsInSystem rdf:type owl:ObjectProperty ;
                 rdfs:domain :Technique ;
                 rdfs:range :StylingSystem ;
                 rdfs:label "belongs in system" .
                 
###  http://semanticweb.org/ont/martialmotion#isFeatureOf
:isFeatureOf rdf:type owl:ObjectProperty ;
             rdfs:range [ rdf:type owl:Class ;
                          owl:unionOf ( :StylingSystem
                                        :Technique
                                      )
                        ] .





###  http://semanticweb.org/ont/martialmotion#symbolicallyRepresents
:symbolicallyRepresents rdf:type owl:ObjectProperty ;
                        rdfs:domain [ rdf:type owl:Class ;
                                      owl:unionOf ( :Choreography
                                                    :StylingSystem
                                                    :Technique
                                                  )
                                    ] ;
                        dct:description "the symbolic binding between a form, technique etc. and a wordly entity, e.g. the relationship between a kata and the combat it simulates, or a crane style with a crane's movements."@en ;
                        rdfs:comment "TODO map to CIDOC CRM symbolic representations or with DOLCE"@en ;
                        rdfs:label "symbolically represents"@en .
                        
###  http://semanticweb.org/ont/martialmotion#AmbiTechnique
:AmbiTechnique rdf:type owl:Class ;
               rdfs:subClassOf :FrontalTechnique ,
                               :ReverseTechnique ;
               dct:description "A technique that has both at least one frontal element and at least one reverse element."@en ;
               rdfs:comment "e.g. holding a staff in the middle and using both ends to attack."@en ;
               rdfs:label "ambivalent technique"@en .

###  http://semanticweb.org/ont/martialmotion#Choreography
:Choreography rdf:type owl:Class ;
              rdfs:subClassOf dul:Method ;
              rdfs:comment "Forms. Examples include Japanese kata, Chinese taolu, Korean hyung, and Southeast Asian jurus (preset) and tari (freeform)"@en ,
                           "TODO: make a separate class for Form?"@en .


###  http://semanticweb.org/ont/martialmotion#DynamicTrainingMethod
:DynamicTrainingMethod rdf:type owl:Class ;
                       rdfs:subClassOf :TrainingMethod ;
                       owl:disjointWith :StaticTrainingMethod ;
                       rdfs:label "dynamic training method" .


###  http://semanticweb.org/ont/martialmotion#EmptyHandTechnique
:EmptyHandTechnique rdf:type owl:Class ;
                    rdfs:subClassOf :Technique ,
                                    [ rdf:type owl:Restriction ;
                                      owl:onProperty :employsArmament ;
                                      owl:allValuesFrom :BodyPartType
                                    ] ;
                    owl:disjointWith :WeaponTechnique .


###  http://semanticweb.org/ont/martialmotion#FrontalTechnique
:FrontalTechnique rdf:type owl:Class ;
                  rdfs:subClassOf :Technique ;
                  rdfs:label "frontal technique" .
                  
###  http://semanticweb.org/ont/martialmotion#HardApproach
:HardApproach rdf:type owl:Class ;
              rdfs:subClassOf :IntentiveApproach ;
              dct:description "An intent that requires hardening of the body prior to the execution of a technique."@en .


###  http://semanticweb.org/ont/martialmotion#IntentiveApproach
:IntentiveApproach rdf:type owl:Class ;
                   dct:description "an approach with an intent (e.g. to attack, distract or defend)"@en ;
                   rdfs:label "intentive approach"@en .

###  http://semanticweb.org/ont/martialmotion#ReverseTechnique
:ReverseTechnique rdf:type owl:Class ;
                  rdfs:subClassOf :Technique ;
                  rdfs:label "reverse technique" .


###  http://semanticweb.org/ont/martialmotion#SoftApproach
:SoftApproach rdf:type owl:Class ;
              rdfs:subClassOf :IntentiveApproach ;
              dct:description "An intent that requires loosening of the body prior to the execution of a technique."@en .


###  http://semanticweb.org/ont/martialmotion#StaticTrainingMethod
:StaticTrainingMethod rdf:type owl:Class ;
                      rdfs:subClassOf :TrainingMethod ;
                      rdfs:label "static training method" .

###  http://semanticweb.org/ont/martialmotion#StylingSystem
:StylingSystem rdf:type owl:Class ;
               rdfs:subClassOf dul:Method ;
               dct:description "Combination of techniques under a common aegis (e.g. Wado-ryu karate, Hakka staff-fighting system)."@en ;
               rdfs:label "styling system"@en .


###  http://semanticweb.org/ont/martialmotion#Technique
:Technique rdf:type owl:Class ;
           rdfs:subClassOf dul:Method ;
           dct:description "What can atomically be considered a technique (e.g. stance, hand form) or combination thereof."@en ;
           rdfs:label "martial technique"@en .


###  http://semanticweb.org/ont/martialmotion#TrainingMethod
:TrainingMethod rdf:type owl:Class ;
                rdfs:subClassOf dul:Method ;
                dct:description "a way of matering a styling system, or a technique therein"@en ;
                rdfs:label "training method" .


###  http://semanticweb.org/ont/martialmotion#TrainingSet
:TrainingSet rdf:type owl:Class ;
             dct:description "A training method (in a technique or for a whole style) may be comprised of separate training sets, e.g. one solo and one for sparring in two or more."@en ;
             rdfs:label "training set" .
             
###  http://semanticweb.org/ont/martialmotion#WeaponTechnique
:WeaponTechnique rdf:type owl:Class ;
                 rdfs:subClassOf :Technique ,
                                 [ rdf:type owl:Restriction ;
                                   owl:onProperty :employsArmament ;
                                   owl:someValuesFrom :WeaponType
                                 ] .
